Added traversal lemmas both for exec_tls and exec_tls_cip

src/travorder/SimIordTraversal.v
@@ -24,6 +24,46 @@ Import ListNotations.
 
 Set Implicit Arguments.
 
+(* TODO: move to TLSCoherency *)
+Lemma init_exec_tls_disjoint G:
+  set_disjoint (init_tls G) (exec_tls G). 
+Proof using. unfold init_tls, exec_tls. iord_dom_unfolder. Qed. 
+
+(* TODO: move to SimClosure *)
+Lemma exec_tls_sim_coh G (WF: Wf G):
+  sim_coherent G (exec_tls G).
+Proof using. 
+  unfold sim_coherent, sim_clos. split; [basic_solver| ].
+  repeat (apply set_subset_union_l; split; try basic_solver). 
+  { unfold rmw_clos, exec_tls, tl_covered, tl_issued.
+    repeat rewrite set_pair_alt.
+    rewrite wf_rmwE, wf_rmwD, rmw_non_init_lr; auto. 
+    iord_dom_unfolder; [by vauto| ]. intuition. }
+  { unfold rel_clos, exec_tls, tl_covered, tl_issued.
+    repeat rewrite set_pair_alt.
+    iord_dom_unfolder. left. vauto. }
+Qed.
+
+(* TODO: move to SimClosure*)
+Lemma init_tls_sim_coh G (WF: Wf G):
+  sim_coherent G (init_tls G).
+Proof using. 
+  unfold sim_coherent, sim_clos. split; [basic_solver| ].
+  repeat (apply set_subset_union_l; split); try basic_solver.
+  { unfold rmw_clos. rewrite set_pair_alt. etransitivity.
+    { red. intro. apply proj2. }
+    iord_dom_unfolder. do 2 red in d. desc. red in d. desc.
+    apply init_tls_EI in d. red in d.
+    apply rmw_non_init_lr, seq_eqv_lr in d0; auto. type_solver. }
+  unfold rel_clos. rewrite set_pair_alt. etransitivity.
+  { red. intro. apply proj2. }
+  iord_dom_unfolder. do 2 red in d. desc. red in d. desc.
+  apply init_tls_EI in d. do 2 red in d. desc.
+  destruct y, a0; try by vauto. ins. subst. 
+  forward eapply (wf_init_lab WF l) as ?.
+  unfold is_rel, Events.mod in c. rewrite H in c. vauto. 
+Qed.
+
 Section IordTraversal. 
   Variable (G: execution) (sc: relation actid). 
   Implicit Types (WF : Wf G) (COMP : complete G)
@@ -104,35 +144,38 @@ Section IordTraversal.
   Section StepsEnum.
     
     Variable (steps: nat -> trav_label).
-    Hypothesis (ENUM: enumerates steps (exec_tls G)).
-    Hypothesis (RESP: respects_rel steps iord⁺ (exec_tls G)).
+    Variable (r: relation trav_label).
+    Variable (dom: trav_label -> Prop).
+    Hypothesis (IORD_DOM: r ⊆ dom × dom).
+    Hypothesis (ENUM: enumerates steps dom).
+    Hypothesis (RESP: respects_rel steps r⁺ dom).
 
     Definition trav_prefix (i: nat) : trav_label -> Prop :=
       ⋃₁ j < i, eq (steps j).
 
-    Lemma trav_prefix_iord_closed WF COMP WFSC CONS
-          i (DOMi: NOmega.le (NOnum i) (set_size (exec_tls G))):
-      dom_rel (iord⁺ ⨾ ⦗trav_prefix i⦘) ⊆₁ trav_prefix i.
-    Proof using ENUM RESP.
+    Lemma trav_prefix_rel_closed WF COMP WFSC CONS
+          i (DOMi: NOmega.le (NOnum i) (set_size dom)):
+      dom_rel (r⁺ ⨾ ⦗trav_prefix i⦘) ⊆₁ trav_prefix i.
+    Proof using ENUM RESP IORD_DOM.
       unfold trav_prefix. 
       red. intros e' [e DOMe']. apply seq_eqv_r in DOMe' as [REL ENUMe].
       red in ENUMe. destruct ENUMe as [j [LTji STEPje]].
       apply enumeratesE' in ENUM. cdes ENUM.
       specialize (IND e'). specialize_full IND.
       { eapply clos_trans_more in REL.
-        2: { symmetry. apply iord_exec_tls. }
-        apply restr_ct in REL. apply REL. }
+        2: { symmetry. apply dom_helper_3. eauto. }
+        apply ct_begin in REL. generalize REL. clear. basic_solver. }
         
       destruct IND as [k [DOMk STEPke']].
       red. exists k. splits; eauto.      
       etransitivity; [| apply LTji].
       red in RESP. apply RESP with (j := j); eauto.
       2: congruence.
-      liaW (set_size (exec_tls G)). 
+      liaW (set_size dom). 
     Qed. 
 
     (* TODO: generalize to arbitrary enumerations? *)
-    Lemma prefix_border i (DOMi: NOmega.lt_nat_l i (set_size (exec_tls G))):
+    Lemma prefix_border i (DOMi: NOmega.lt_nat_l i (set_size dom)):
       ~ trav_prefix i (steps i).
     Proof using ENUM.
       unfold trav_prefix. intros [j [LT EQ]]. 
@@ -141,17 +184,23 @@ Section IordTraversal.
       eapply NOmega.lt_lt_nat; eauto.
     Qed.
 
-    Lemma step_event_dom i (DOMi: NOmega.lt_nat_l i (set_size (exec_tls G))):
-      (E \₁ is_init) (event (steps i)) /\
-      (action (steps i) = ta_issue -> W (event (steps i))). 
-    Proof using ENUM. 
+    (* Lemma step_event_dom i (DOMi: NOmega.lt_nat_l i (set_size dom)): *)
+    (*   (E \₁ is_init) (event (steps i)) /\ *)
+    (*   (action (steps i) = ta_issue -> W (event (steps i))).  *)
+    (* Proof using ENUM.  *)
+    (*   apply enumeratesE' in ENUM. cdes ENUM. *)
+    (*   specialize_full INSET; eauto. red in INSET. *)
+    (*   destruct (steps i) as [a e]. unfolder in INSET. basic_solver.  *)
+    (* Qed.  *)
+    Lemma step_event_dom i (DOMi: NOmega.lt_nat_l i (set_size dom)):
+      dom (steps i). 
+    Proof using ENUM.
       apply enumeratesE' in ENUM. cdes ENUM.
-      specialize_full INSET; eauto. red in INSET.
-      destruct (steps i) as [a e]. unfolder in INSET. basic_solver. 
-    Qed. 
+      specialize_full INSET; eauto. 
+    Qed.       
 
     Lemma trav_prefix_ext i
-          (DOMi: NOmega.lt_nat_l i (set_size (exec_tls G))):
+          (DOMi: NOmega.lt_nat_l i (set_size dom)):
       trav_prefix (S i) ≡₁ trav_prefix i ∪₁ eq (steps i).
     Proof using. 
       unfold trav_prefix.
@@ -160,38 +209,30 @@ Section IordTraversal.
       rewrite set_bunion_union_l. basic_solver.
     Qed.
 
-(* End IordTraversal.  *)
-
-(* Section Traversal. *)
-(*   Variable (steps: nat -> trav_label). *)
-(*   Hypothesis (ENUM: enumerates steps (exec_tls G)). *)
-(*   Hypothesis (RESP: respects_rel steps (iord G sc)⁺ (exec_tls G)). *)
-  
-  Definition tc_enum (i: nat): trav_label -> Prop  :=
-    sim_clos G (trav_prefix i) ∪₁ init_tls G. 
-  
   Lemma trav_prefix_init:
     trav_prefix 0 ≡₁ ∅. 
-  Proof.
+  Proof using.
     unfold trav_prefix. apply set_subset_empty_r, set_subset_bunion_l.
     ins. lia. 
   Qed.
-    
-  Lemma trav_prefix_iord_coherent 
-        (i : nat) (DOMi: NOmega.le (NOnum i) (set_size (exec_tls G))):
-    iord_coherent G sc (trav_prefix i).
-  Proof using RESP ENUM.
+  
+  Lemma trav_prefix_r_closed 
+        (i : nat) (DOMi: NOmega.le (NOnum i) (set_size dom)):
+    dom_rel (r ⨾ ⦗trav_prefix i⦘) ⊆₁ trav_prefix i.
+  Proof using RESP ENUM IORD_DOM.
     induction i.
     { rewrite trav_prefix_init. red. basic_solver. }
-    rewrite trav_prefix_ext; eauto. red.
+    rewrite trav_prefix_ext; eauto. 
     rewrite id_union, seq_union_r, dom_union.
     apply set_subset_union_l. split. 
     { unfold iord_coherent in IHi. rewrite IHi; [basic_solver| ].
-      liaW (set_size (exec_tls G)). }
+      liaW (set_size dom). }
     red. intros tlj. intros [tli IORD%seq_eqv_r]. desc.
-    apply iord_exec_tls in IORD. red in IORD. desc.
+    (* apply iord_exec_tls in IORD. red in IORD. desc. *)
+    apply dom_helper_3 in IORD_DOM.
+    apply IORD_DOM, seq_eqv_lr in IORD as (Dj & Rji & Di).  
     apply enumeratesE' in ENUM. cdes ENUM.
-    apply IND in IORD1, IORD2. desc. rename i1 into j.
+    apply IND in Dj, Di. desc. rename i1 into j.
     assert (i0 = i) as -> by (apply INJ; auto; congruence).
     subst. 
     pose proof (Nat.lt_trichotomy i j) as LT. des; revgoals. 
@@ -201,136 +242,127 @@ Section IordTraversal.
     enough (j < i); [lia| ]. eapply RESP; eauto; try by apply ct_step.
   Qed.
   
-  Lemma trav_prefix_step
-        i (DOMsi: NOmega.lt_nat_l i (set_size (exec_tls G))):
-    iord_step G sc (trav_prefix i) (trav_prefix (S i)).
-  Proof using RESP ENUM.
-    red. exists (steps i). do 2 red.
-    splits; try by (apply trav_prefix_iord_coherent; liaW (set_size (exec_tls G))).
-    apply seq_eqv_l. split.
-    { eapply prefix_border; eauto. }
-    eapply trav_prefix_ext; eauto. 
-  Qed.
-
-  Lemma init_tls_sim_coh WF:
-    sim_coherent G (init_tls G).
-  Proof. 
-    unfold sim_coherent, sim_clos. split; [basic_solver| ].
-    repeat (apply set_subset_union_l; split); try basic_solver.
-    { unfold rmw_clos. rewrite set_pair_alt. etransitivity.
-      { red. intro. apply proj2. }
-      iord_dom_unfolder. do 2 red in d. desc. red in d. desc.
-      apply init_tls_EI in d. red in d.
-      apply rmw_non_init_lr, seq_eqv_lr in d0; auto. type_solver. }
-    { unfold rel_clos. rewrite set_pair_alt. etransitivity.
-      { red. intro. apply proj2. }
-      iord_dom_unfolder. do 2 red in d. desc. red in d. desc.
-      apply init_tls_EI in d. do 2 red in d. desc.
-      destruct y, a0; try by vauto. ins. subst. 
-      forward eapply (wf_init_lab WF l) as ?.
-      unfold is_rel, Events.mod in c. rewrite H in c. vauto. }
-  Qed.
-
-  (* TODO: group similar lemmas about union with init_tls *)
-  Lemma trav_prefix_init_tls_iord_coherent i
-        (DOMi : NOmega.le (NOnum i) (set_size (exec_tls G))):
-    iord_coherent G sc (trav_prefix i ∪₁ init_tls G).
-  Proof.
-    red. unfold tc_enum. rewrite id_union, seq_union_r, dom_union.
-    apply set_subset_union_l. split.
-    { apply set_subset_union_r. left. apply trav_prefix_iord_coherent; auto. }
-    unfold "iord". rewrite init_tls_EI at 1. basic_solver.
-  Qed. 
-
-  (* TODO: move upper *)
-  Lemma init_exec_tls_disjoint:
-    set_disjoint (init_tls G) (exec_tls G). 
-  Proof. unfold init_tls, exec_tls. iord_dom_unfolder. Qed. 
-
-  Lemma trav_prefix_in_exec_tls i
-        (DOMi: NOmega.le (NOnum i) (set_size (exec_tls G))):
-    trav_prefix i ⊆₁ exec_tls G. 
-  Proof. 
+  Lemma trav_prefix_in_dom i
+        (DOMi: NOmega.le (NOnum i) (set_size dom)):
+    trav_prefix i ⊆₁ dom. 
+  Proof using ENUM. 
     apply enumeratesE' in ENUM. cdes ENUM. 
     unfold trav_prefix. apply set_subset_bunion_l. intros.
     apply set_subset_single_l. apply INSET.
-    liaW (set_size (exec_tls G)). 
+    liaW (set_size dom). 
   Qed.
 
+  End StepsEnum.
+
+  Section IordEnum.
+    (* This generalization is used to support traversal 
+       of both complete exec_tls and its parts *)
+
+  Variable (steps: nat -> trav_label).
+  Variable (dom: trav_label -> Prop).
+  Hypothesis (IORD_DOM: iord ⊆ dom × dom).
+  Hypothesis (DOM_EXEC: dom ⊆₁ exec_tls G). 
+  Hypothesis (ENUM: enumerates steps dom).
+  Hypothesis (RESP: respects_rel steps iord⁺ dom).
+
+  Lemma trav_prefix_in_exec_tls i
+        (DOMi: NOmega.le (NOnum i) (set_size dom)):
+    trav_prefix steps i ⊆₁ exec_tls G. 
+  Proof using ENUM DOM_EXEC. 
+    apply enumeratesE' in ENUM. cdes ENUM. 
+    unfold trav_prefix. apply set_subset_bunion_l. intros.
+    rewrite <- DOM_EXEC. apply set_subset_single_l. apply INSET.
+    liaW (set_size dom). 
+  Qed.
+
+  Lemma trav_prefix_step
+        i (DOMsi: NOmega.lt_nat_l i (set_size dom)):
+    iord_step G sc (trav_prefix steps i) (trav_prefix steps (S i)).
+  Proof using RESP ENUM IORD_DOM.
+    red. exists (steps i). do 2 red.
+    splits; try by (red; eapply trav_prefix_r_closed; eauto; liaW (set_size dom)).
+    apply seq_eqv_l. split.
+    { eapply prefix_border; eauto. }
+    eapply trav_prefix_ext; eauto.
+  Qed.
+
+  Definition tc_enum (i: nat): trav_label -> Prop  :=
+    sim_clos G (trav_prefix steps i) ∪₁ init_tls G. 
+  
+  (* TODO: group similar lemmas about union with init_tls *)
+  Lemma trav_prefix_init_tls_iord_coherent i
+        (DOMi : NOmega.le (NOnum i) (set_size dom)):
+    iord_coherent G sc (trav_prefix steps i ∪₁ init_tls G).
+  Proof using RESP IORD_DOM ENUM.
+    red. rewrite id_union, seq_union_r, dom_union.
+    apply set_subset_union_l. split.
+    { apply set_subset_union_r. left. eapply trav_prefix_r_closed; eauto. }
+    unfold "iord". rewrite init_tls_EI at 1. basic_solver.
+  Qed.
+
+  Lemma tc_enum_tls_coherent WF i
+      (DOMi: NOmega.le (NOnum i) (set_size dom)):
+    tls_coherent G (tc_enum i). 
+  Proof using ENUM DOM_EXEC.
+    unfold tc_enum. split; [basic_solver| ].
+    apply set_subset_union_l. split; [| basic_solver].
+    erewrite sim_clos_mori.
+    2: { apply trav_prefix_in_exec_tls; eauto. }
+    pose proof (exec_tls_sim_coh WF). red in H. rewrite <- H. basic_solver. 
+  Qed.
+
+  Lemma trav_prefix_union_init_tls_coherent WF i
+      (DOMi: NOmega.le (NOnum i) (set_size dom)):
+    tls_coherent G (trav_prefix steps i ∪₁ init_tls G). 
+  Proof using ENUM DOM_EXEC. 
+    apply tls_coherent_defs_equiv. exists (trav_prefix steps i).
+    split; [| basic_solver]. now apply trav_prefix_in_exec_tls.
+  Qed. 
+
   Lemma trav_prefix_step_ext
-        i (DOMsi: NOmega.lt_nat_l i (set_size (exec_tls G))):
-    iord_step G sc (trav_prefix i ∪₁ init_tls G)
-              (trav_prefix (S i) ∪₁ init_tls G). 
-  Proof. 
+        i (DOMsi: NOmega.lt_nat_l i (set_size dom)):
+    iord_step G sc (trav_prefix steps i ∪₁ init_tls G)
+              (trav_prefix steps (S i) ∪₁ init_tls G). 
+  Proof using RESP IORD_DOM ENUM DOM_EXEC. 
     forward eapply trav_prefix_step as [l STEP]; eauto.
     red. exists l. do 2 red.
-    splits; try by (apply trav_prefix_init_tls_iord_coherent; liaW (set_size (exec_tls G))).
+    splits; try by (apply trav_prefix_init_tls_iord_coherent; liaW (set_size dom)).
     do 2 red in STEP. desc. apply seq_eqv_l in STEP. desc.  
     apply seq_eqv_l. split.
     2: { rewrite STEP2. basic_solver. }
     apply set_compl_union. split; auto.
     apply set_disjoint_eq_r. eapply set_disjoint_mori; [reflexivity| ..].
     2: by apply init_exec_tls_disjoint.
-    red. rewrite <- (@trav_prefix_in_exec_tls (S i)); auto.
-    rewrite STEP2. basic_solver. 
-  Qed. 
-  
-  (* TODO: move upper *)
-  Lemma exec_tls_sim_coh WF:
-    sim_coherent G (exec_tls G).
-  Proof. 
-    unfold sim_coherent, sim_clos. split; [basic_solver| ].
-    repeat (apply set_subset_union_l; split; try basic_solver). 
-    { unfold rmw_clos, exec_tls, tl_covered, tl_issued.
-      repeat rewrite set_pair_alt.
-      rewrite wf_rmwE, wf_rmwD, rmw_non_init_lr; auto. 
-      iord_dom_unfolder; [by vauto| ]. 
-      right. eauto. }
-    { unfold rel_clos, exec_tls, tl_covered, tl_issued.
-      repeat rewrite set_pair_alt.
-      iord_dom_unfolder. left. vauto. }
-  Qed. 
-
-  Lemma tc_enum_tls_coherent WF i
-      (DOMi: NOmega.le (NOnum i) (set_size (exec_tls G))):
-    tls_coherent G (tc_enum i). 
-  Proof.
-    unfold tc_enum. split; [basic_solver| ].
-    apply set_subset_union_l. split; [| basic_solver].
-    erewrite sim_clos_mori.
-    2: { apply trav_prefix_in_exec_tls. auto. }
-    pose proof (exec_tls_sim_coh WF). red in H. rewrite <- H. basic_solver. 
-  Qed.
-
-  Lemma trav_prefix_union_init_tls_coherent WF i
-      (DOMi: NOmega.le (NOnum i) (set_size (exec_tls G))):
-    tls_coherent G (trav_prefix i ∪₁ init_tls G). 
-  Proof using ENUM. 
-    apply tls_coherent_defs_equiv. exists (trav_prefix i). split; [| basic_solver].
-    apply trav_prefix_in_exec_tls. auto. 
+    red. rewrite <- DOM_EXEC.
+    forward eapply @trav_prefix_in_dom with (i := S i) as XX; eauto.
+    rewrite <- XX. rewrite STEP2. basic_solver. 
   Qed. 
 
   Lemma sim_traversal_next WF CONS:
-    forall i (DOMi: NOmega.lt_nat_l i (set_size (exec_tls G))),
+    forall i (DOMi: NOmega.lt_nat_l i (set_size dom)),
       (sim_clos_step G sc)^* (tc_enum i) (tc_enum (1 + i)). 
-  Proof using RESP ENUM.
+  Proof using RESP ENUM IORD_DOM DOM_EXEC.
     ins. unfold tc_enum.
-    forward eapply init_tls_sim_coh as INIT_SCOH; auto. red in INIT_SCOH.
+    forward eapply init_tls_sim_coh as INIT_SCOH; eauto. red in INIT_SCOH.
     rewrite INIT_SCOH, <- !sim_clos_dist; auto.  
     apply iord_step_implies_sim_clos_step; auto.
-    red. splits; try by (apply trav_prefix_union_init_tls_coherent; liaW (set_size (exec_tls G))). 
+    red. splits; try by (apply trav_prefix_union_init_tls_coherent; liaW (set_size dom)). 
     apply trav_prefix_step_ext; auto. 
   Qed.
 
-  End StepsEnum.
+  End IordEnum. 
+
 
   Lemma iord_enum_exists WF COMP WFSC CONS MF
-        (IMM_FAIR: imm_s_fair G sc):
+        (IMM_FAIR: imm_s_fair G sc)
+        dom
+        (* (IORD_DOM: iord ⊆ dom × dom) (DOM_EXEC: dom ⊆₁ exec_tls G) *)
+    :
   exists (steps: nat -> trav_label),
-    enumerates steps (exec_tls G) /\
-      respects_rel steps iord⁺ (exec_tls G). 
+    enumerates steps dom /\
+    respects_rel steps iord⁺ dom. 
   Proof using.
-    edestruct countable_ext with (s := exec_tls G) (r := ⦗event ↓₁ (set_compl is_init)⦘ ⨾ iord⁺)
+    edestruct countable_ext with (s := dom) (r := ⦗event ↓₁ (set_compl is_init)⦘ ⨾ iord⁺)
       as [| [steps [ENUM RESP]]].
     { eapply countable_subset; [| by apply set_subset_full_r].
       apply trav_label_countable. }
@@ -345,11 +377,154 @@ Section IordTraversal.
     1, 2: by apply set_lt_size.
     apply seq_eqv_l. split; auto.
     apply enumeratesE' in ENUM. desc. apply INSET in DOMi.
-    red in DOMi. clear -DOMi. unfold set_pair in *. unfolder in DOMi. desf; desf.
+    apply ct_begin in Rij. generalize Rij. unfold iord. basic_solver. 
   Qed.
-  
+
+
   (* TODO: rename? *)
   Lemma sim_traversal_inf WF CONS
+        (FAIR: mem_fair G)
+        (IMM_FAIR: imm_s_fair G sc)
+        (dom: trav_label -> Prop)
+        (IORD_DOM: iord ⊆ dom × dom)
+        (DOM_EXEC: dom ⊆₁ exec_tls G)
+        (DOM_COVERS: eq ta_cover <*> (E \₁ is_init) ⊆₁ dom)
+        (DOM_SIM_CLOSURE: forall (S: trav_label -> Prop) (S_DOM: S ⊆₁ dom),
+            (@sim_clos G S) ⊆₁ dom):
+    exists (sim_enum: nat -> (trav_label -> Prop)),
+      ⟪INIT: sim_enum 0 ≡₁ init_tls G ⟫ /\
+      ⟪COH: forall i (DOMi: NOmega.le (NOnum i) (set_size dom)),
+          tls_coherent G (sim_enum i)⟫ /\
+      ⟪STEPS: forall i (DOMi: NOmega.lt_nat_l i (set_size dom)),
+          (sim_clos_step G sc)^* (sim_enum i) (sim_enum (1 + i)) ⟫ /\
+      ⟪ENUM: forall e (Ee: (E \₁ is_init) e), exists i,
+           NOmega.le (NOnum i) (set_size dom) /\
+             (sim_enum i) (mkTL ta_cover e)⟫ /\
+      ⟪DOM: forall i (DOMi: NOmega.le (NOnum i) (set_size dom)),
+          sim_enum i ⊆₁ init_tls G ∪₁ dom⟫.
+  Proof using.
+    edestruct iord_enum_exists as [steps_enum [ENUM RESP]]; eauto.
+    1, 2: by apply CONS.
+    exists (tc_enum steps_enum). splits.
+    { unfold tc_enum. rewrite trav_prefix_init.
+      rewrite sim_clos_empty. basic_solver. }
+    { apply tc_enum_tls_coherent; eauto. }
+    { apply sim_traversal_next; auto. }
+    { intros e Ee.
+      pose proof ENUM as ENUM'. apply enumeratesE' in ENUM. desc.
+      specialize (IND (mkTL ta_cover e)). specialize_full IND. 
+      { apply DOM_COVERS. vauto. } 
+      desc. exists (S i). split; [by vauto| ].  
+      eapply set_equiv_exp. 
+      { unfold tc_enum. rewrite trav_prefix_ext; eauto. }
+      rewrite IND0. unfold sim_clos. basic_solver 10.  }
+    ins. unfold tc_enum. rewrite set_unionC. apply set_subset_union; [done| ]. 
+    rewrite <- DOM_SIM_CLOSURE; [reflexivity| ]. 
+    eapply trav_prefix_in_dom; eauto.
+  Qed.
+
+  Lemma exec_tls_cip_alt:
+    exec_tls_cip G ≡₁ exec_tls G \₁ action ↓₁ eq ta_reserve. 
+  Proof using. 
+    unfold exec_tls_cip, exec_tls. rewrite !set_pair_alt.
+    split; try basic_solver 10.
+    rewrite set_minus_union_l.
+    unfolder. ins. destruct x; ins; des; subst; splits; try by vauto.
+    { right. splits; vauto. }
+    do 2 red in H. desc. subst. right. splits; vauto. 
+  Qed. 
+
+  (* TODO: move *)
+  Lemma iord_exec_tls_cip:
+    iord ⊆ exec_tls_cip G × exec_tls_cip G. 
+  Proof using.
+    rewrite exec_tls_cip_alt, set_minusE.
+    rewrite restr_rel_cross_inter.
+    split.
+    { eapply iord_exec_tls; eauto. }
+    do 2 red in H. desc. clear -H. unfolder in H. des.
+    all: apply seq_eqv_lr in H as (X & _ & Y); red in X, Y; vauto;
+      split; red; intros [=]; try congruence.
+    { do 2 red in Y. desc. congruence. }
+    { do 2 red in Y. desc. congruence. } 
+  Qed. 
+
+  Lemma rmw_clos_exec_tls tc (WF: Wf G):
+    rmw_clos G tc ⊆₁ exec_tls G. 
+  Proof using.
+    unfold rmw_clos, exec_tls. rewrite !set_pair_alt.
+    arewrite (codom_rel (⦗tl_covered tc⦘ ⨾ rmw) ⊆₁ (E \₁ is_init) ∩₁ W).
+    2: { basic_solver 10. }
+    rewrite wf_rmwD, wf_rmwE, rmw_in_sb, no_sb_to_init; auto. basic_solver.
+  Qed. 
+  
+  Lemma rel_clos_exec_tls tc (WF: Wf G) (TC_E: tc ⊆₁ event ↓₁ E):
+    rel_clos G tc ⊆₁ exec_tls G.
+  Proof using.
+    unfold rel_clos, exec_tls. rewrite !set_pair_alt.
+    apply set_subset_union_r. left. apply set_subset_inter; [done| ].
+    apply set_map_mori; [done| ]. unfold tl_issued.
+    unfolder. ins. desc. split.
+    { apply TC_E in H0. vauto. }
+    eintros INIT%init_pln; eauto. mode_solver.
+  Qed.
+  
+  Lemma sim_clos_exec_tls WF tc
+        (TC_EXEC: tc ⊆₁ exec_tls G):
+    sim_clos G tc ⊆₁ exec_tls G. 
+  Proof using.
+    repeat (apply set_subset_union_l; split); auto.
+    { by apply rmw_clos_exec_tls. }
+    apply rel_clos_exec_tls; auto. rewrite TC_EXEC.
+    rewrite exec_tls_ENI. basic_solver. 
+  Qed.
+  
+  (* TODO: replace original proof with this + lemmas above *)
+  Lemma sim_clos_tls_coherent' WF tc
+        (TCOH: tls_coherent G tc):
+    tls_coherent G (sim_clos G tc). 
+  Proof using.
+    pose proof TCOH as TCOH'.
+    apply tls_coherent_defs_equiv. apply tls_coherent_defs_equiv in TCOH.
+    red in TCOH. desc.
+    red. unfold sim_clos. exists (tc' ∪₁ rmw_clos G tc ∪₁ rel_clos G tc). split.
+    2: { rewrite TCOH0 at 1. basic_solver. }
+    repeat (apply set_subset_union_l; split); auto.
+    { by apply rmw_clos_exec_tls. }
+    apply rel_clos_exec_tls; auto. by apply tlsc_E. 
+  Qed.  
+
+  (* TODO: rename? *)
+  Lemma sim_traversal_inf_cip WF CONS
+        (FAIR: mem_fair G)
+        (IMM_FAIR: imm_s_fair G sc)
+        :
+    exists (sim_enum: nat -> (trav_label -> Prop)),
+      ⟪INIT: sim_enum 0 ≡₁ init_tls G ⟫ /\
+      ⟪COH: forall i (DOMi: NOmega.le (NOnum i) (set_size (exec_tls_cip G))),
+          tls_coherent G (sim_enum i)⟫ /\
+      ⟪STEPS: forall i (DOMi: NOmega.lt_nat_l i (set_size (exec_tls_cip G))),
+          (sim_clos_step G sc)^* (sim_enum i) (sim_enum (1 + i)) ⟫ /\
+      ⟪ENUM: forall e (Ee: (E \₁ is_init) e), exists i,
+           NOmega.le (NOnum i) (set_size (exec_tls_cip G)) /\
+             (sim_enum i) (mkTL ta_cover e)⟫ /\
+      ⟪DOM: forall i (DOMi: NOmega.le (NOnum i) (set_size (exec_tls_cip G))),
+          sim_enum i ⊆₁ init_tls G ∪₁ exec_tls_cip G⟫.
+  Proof using.
+    forward eapply sim_traversal_inf with (dom := exec_tls_cip G) as TRAV; eauto.
+    { apply iord_exec_tls_cip. }
+    { unfold exec_tls_cip, exec_tls. rewrite !set_pair_alt. basic_solver 10. }
+    { unfold exec_tls_cip, exec_tls. rewrite !set_pair_alt. basic_solver 10. }
+    ins. rewrite exec_tls_cip_alt, set_minusE. apply set_subset_inter_r. split.
+    { apply sim_clos_exec_tls; auto. rewrite S_DOM.
+      rewrite exec_tls_cip_alt. basic_solver. }
+    unfold sim_clos. repeat (apply set_subset_union_l; split).
+    2, 3: unfold rmw_clos, rel_clos; iord_dom_solver. 
+    rewrite S_DOM, exec_tls_cip_alt. basic_solver. 
+  Qed.
+
+  (* TODO: rename? *)
+  Lemma sim_traversal_inf_full WF CONS
         (FAIR: mem_fair G)
         (IMM_FAIR: imm_s_fair G sc):
     exists (sim_enum: nat -> (trav_label -> Prop)),
@@ -362,24 +537,11 @@ Section IordTraversal.
            NOmega.le (NOnum i) (set_size (exec_tls G)) /\
              (sim_enum i) (mkTL ta_cover e)⟫.
   Proof using.
-    edestruct iord_enum_exists as [steps_enum [ENUM RESP]]; eauto.
-    1, 2: by apply CONS.
-    exists (tc_enum steps_enum). splits.
-    { unfold tc_enum. rewrite trav_prefix_init.
-      rewrite sim_clos_empty. basic_solver. }
-    { apply tc_enum_tls_coherent; auto. }
-    { apply sim_traversal_next; auto. }
-    
-    intros e Ee.
-    pose proof ENUM as ENUM'. apply enumeratesE' in ENUM. desc.
-    specialize (IND (mkTL ta_cover e)). specialize_full IND; [by vauto| ].
-    desc. exists (S i). split; [by vauto| ].  
-    eapply set_equiv_exp. 
-    { unfold tc_enum. rewrite trav_prefix_ext; auto. }
-    rewrite IND0. unfold sim_clos. basic_solver 10.  
+    forward eapply sim_traversal_inf with (dom := exec_tls G) as TRAV; eauto.
+    { rewrite iord_exec_tls. basic_solver. }
+    { unfold exec_tls. basic_solver. }
+    { ins. apply sim_clos_exec_tls; auto. }
+    desc. eexists. splits; eauto. 
   Qed.
 
 End IordTraversal.
-
-  
-
